Update PER

theories/Core/Semantic/PER.v
@@ -1,4 +1,6 @@
-From Coq Require Import Lia PeanoNat Relations Program.Wf.
+From Coq Require Import Lia PeanoNat Relations.
+From Equations Require Import Equations.
+
 From Mcltt Require Import Base Domain Evaluate Readback Syntax System.
 
 Definition in_dom_rel {A} (R : relation A) := R.
@@ -53,7 +55,7 @@ Section Per_univ_elem_core_def.
   | per_univ_elem_core_pi :
     `{ forall (in_rel : relation domain)
           (out_rel : forall {c c'}, {{ Dom c ≈ c' ∈ in_rel }} -> relation domain)
-          (equiv_a_a' : {{ DF a ≈ a' ∈ per_univ_elem_core ↘ in_rel}}),
+          (equiv_a_a' : {{ DF a ≈ a' ∈ per_univ_elem_core ↘ in_rel }}),
           (forall {c c'} (equiv_c_c' : {{ Dom c ≈ c' ∈ in_rel }}),
               rel_mod_eval per_univ_elem_core B d{{{ p ↦ c }}} B' d{{{ p' ↦ c' }}} (out_rel equiv_c_c')) ->
           (elem_rel = fun f f' => forall {c c'} (equiv_c_c' : in_rel c c'),
@@ -66,12 +68,9 @@ End Per_univ_elem_core_def.
 
 Global Hint Constructors per_univ_elem_core : mcltt.
 
-Definition per_univ_like (R : domain -> domain -> relation domain -> Prop) := fun a a' => exists R', {{ DF a ≈ a' ∈ R ↘ R' }}.
-#[global]
-Transparent per_univ_like.
-
-Program Fixpoint per_univ_elem (i : nat) {wf lt i} : domain -> domain -> relation domain -> Prop := Per_univ_def.per_univ_elem i (fun _ lt_j_i => per_univ_like (per_univ_elem _ lt_j_i)).
-Definition per_univ (i : nat) : relation domain := per_univ_like (per_univ_elem i).
+Equations per_univ_elem (i : nat) : domain -> domain -> relation domain -> Prop by wf i :=
+| i => per_univ_elem_core i (fun j lt_j_i a a' => exists R', per_univ_elem j a a' R').
+Definition per_univ (i : nat) : relation domain := fun a a' => exists R', per_univ_elem i a a' R'.
 
 Definition rel_typ (i : nat) (A : typ) (p : env) (A' : typ) (p' : env) R' := rel_mod_eval (per_univ_elem i) A p A' p' R'.
 
@@ -82,8 +81,8 @@ Inductive per_ctx_env : ctx -> ctx -> relation env -> Prop :=
 | per_ctx_env_cons :
   `{ forall (tail_rel : relation env)
         (head_rel : forall {p p'}, {{ Dom p ≈ p' ∈ tail_rel }} -> relation domain)
-        (equiv_Γ_Γ' : {{ EF Γ ≈ Γ' ∈ per_ctx_env ↘ tail_rel }})
-        (rel_A_A' : forall {p p'} (equiv_p_p' : {{ Dom p ≈ p' ∈ tail_rel }}), rel_typ i A p A' p' (head_rel equiv_p_p')),
+        (equiv_Γ_Γ' : {{ EF Γ ≈ Γ' ∈ per_ctx_env ↘ tail_rel }}),
+        (forall {p p'} (equiv_p_p' : {{ Dom p ≈ p' ∈ tail_rel }}), rel_typ i A p A' p' (head_rel equiv_p_p')) ->
         (Env = fun p p' => exists (equiv_p_drop_p'_drop : {{ Dom p ↯ ≈ p' ↯ ∈ tail_rel }}),
                    {{ Dom ~(p 0) ≈ ~(p' 0) ∈ head_rel equiv_p_drop_p'_drop }}) ->
         {{ EF Γ, A ≈ Γ', A' ∈ per_ctx_env ↘ Env }} }
