theories/Core/Semantic/PERLemmas.v
@@ -1,141 +1,44 @@
 From Coq Require Import Lia PeanoNat Relations Program.Equality.
 From Mcltt Require Import Base Domain Evaluate LibTactics PER Readback Syntax System.
-
-(* Lemma per_univ_univ : forall {i j j'}, *)
-(*     j < i -> *)
-(*     j = j' -> *)
-(*     {{ Dom 𝕌@j ≈ 𝕌@j' ∈ per_univ i }}. *)
-(* Proof with solve [mauto]. *)
-(*   intros * lt_j_i eq_j_j'. *)
-(*   eexists... *)
-(*   Unshelve. *)
-(*   all: assumption. *)
-(* Qed. *)
-
-(* Lemma per_univ_nat : forall {i}, *)
-(*     {{ Dom ℕ ≈ ℕ ∈ per_univ i }}. *)
-(* Proof with solve [mauto]. *)
-(*   intros *. *)
-(*   eexists... *)
-(* Qed. *)
-
-(* Lemma per_univ_pi_lem : forall {i a a' B p B' p'} *)
-(*                            (equiv_a_a' : {{ Dom a ≈ a' ∈ per_univ i }}), *)
-(*     (forall {c c'}, *)
-(*         {{ Dom c ≈ c' ∈ per_elem equiv_a_a' }} -> *)
-(*         rel_mod_eval (per_univ i) B d{{{ p ↦ c }}} B' d{{{ p' ↦ c' }}}) -> *)
-(*     exists (rel_B_B'_template : forall {c c'}, *)
-(*         {{ Dom c ≈ c' ∈ per_elem equiv_a_a' }} -> *)
-(*         rel_mod_eval (Per_univ_def.per_univ_template i) B d{{{ p ↦ c }}} B' d{{{ p' ↦ c' }}}), *)
-(*       (forall c c' (equiv_c_c' : {{ Dom c ≈ c' ∈ per_elem equiv_a_a' }}) *)
-(*           b b' (eval_B : {{ ⟦ B ⟧ p ↦ c ↘ b }}) (eval_B' : {{ ⟦ B' ⟧ p' ↦ c' ↘ b' }}), *)
-(*           Per_univ_def.per_univ_check i (@per_univ_base i) (rel_mod_eval_equiv (rel_B_B'_template equiv_c_c') eval_B eval_B')). *)
-(* Proof with solve [mauto]. *)
-(*   intros * rel_B_B'. *)
-(*   unshelve epose (rel_B_B'_template := _ : forall {c c'}, *)
-(*              {{ Dom c ≈ c' ∈ per_elem equiv_a_a' }} -> *)
-(*              rel_mod_eval (Per_univ_def.per_univ_template i) B d{{{ p ↦ c }}} B' d{{{ p' ↦ c' }}}). *)
-(*   { *)
-(*     intros * equiv_c_c'. *)
-(*     econstructor; destruct (rel_B_B' _ _ equiv_c_c') as [? ? ?]; only 1-2: solve [mauto]. *)
-(*     intros b b' eval_B eval_B'. *)
-(*     eapply ex_proj1, rel_mod_eval_equiv... *)
-(*   } *)
-(*   simpl in rel_B_B'_template. *)
-(*   exists rel_B_B'_template. *)
-(*   intros *. *)
-(*   unfold rel_B_B'_template; simpl. *)
-(*   destruct (rel_B_B' _ _ equiv_c_c') as [? ? ?]. *)
-(*   eapply ex_proj2. *)
-(* Qed. *)
-
-(* Lemma per_univ_pi : forall {i a a' B p B' p'} *)
-(*                        (equiv_a_a' : {{ Dom a ≈ a' ∈ per_univ i }}), *)
-(*       (forall {c c'}, *)
-(*           {{ Dom c ≈ c' ∈ per_elem equiv_a_a' }} -> *)
-(*           rel_mod_eval (per_univ i) B d{{{ p ↦ c }}} B' d{{{ p' ↦ c' }}}) -> *)
-(*       {{ Dom Π a p B ≈ Π a' p' B' ∈ per_univ i }}. *)
-(* Proof with solve [mauto]. *)
-(*   intros *; destruct equiv_a_a' as [equiv_a_a'_template equiv_a_a'_check]; intro rel_B_B'. *)
-(*   eassert (H_per_univ_pi_lem : _). *)
-(*   { eapply per_univ_pi_lem... } *)
-(*   destruct H_per_univ_pi_lem as [rel_B_B'_template rel_B_B'_check]. *)
-(*   eexists; econstructor... *)
-(* Qed. *)
-
-(* Lemma per_univ_neut : forall {i m m' a a'}, *)
-(*     {{ Dom m ≈ m' ∈ per_bot }} -> *)
-(*     {{ Dom ⇑ a m ≈ ⇑ a' m' ∈ per_univ i }}. *)
-(* Proof with solve [mauto]. *)
-(*   intros * equiv_m_m'. *)
-(*   eexists... *)
-(*   Unshelve. *)
-(*   all: assumption. *)
-(* Qed. *)
-
-(* Lemma per_univ_ind : forall i P, *)
-(*     (forall j j', j < i -> j = j' -> {{ Dom 𝕌@j ≈ 𝕌@j' ∈ P }}) -> *)
-(*     {{ Dom ℕ ≈ ℕ ∈ P }} -> *)
-(*     (forall a a' B p B' p' *)
-(*         (equiv_a_a' : {{ Dom a ≈ a' ∈ per_univ i }}), *)
-(*         {{ Dom a ≈ a' ∈ P }} -> *)
-(*         (forall c c', *)
-(*             {{ Dom c ≈ c' ∈ per_elem equiv_a_a' }} -> *)
-(*             rel_mod_eval (per_univ i) B d{{{ p ↦ c}}} B' d{{{ p' ↦ c'}}}) -> *)
-(*         (forall {c c'} (equiv_c_c' : {{ Dom c ≈ c' ∈ per_elem equiv_a_a' }}), *)
-(*             rel_mod_eval P B d{{{ p ↦ c}}} B' d{{{ p' ↦ c'}}}) -> *)
-(*         {{ Dom Π a p B ≈ Π a' p' B' ∈ P }}) -> *)
-(*     (forall m m' a a', {{ Dom m ≈ m' ∈ per_bot }} -> {{ Dom ⇑ a m ≈ ⇑ a' m' ∈ P }}) -> *)
-(*     forall d d', {{ Dom d ≈ d' ∈ per_univ i }} -> {{ Dom d ≈ d' ∈ P }}. *)
-(* Proof with solve [mauto]. *)
-(*   intros * Huniv Hnat Hpi Hneut d d' [equiv_d_d'_template equiv_d_d'_check]. *)
-(*   induction equiv_d_d'_check; only 1-2,4: solve [mauto]. *)
-(*   unshelve epose (equiv_a_a'_real := _ : {{ Dom a ≈ a' ∈ per_univ i }}). *)
-(*   { econstructor... } *)
-(*   eapply Hpi with (equiv_a_a' := equiv_a_a'_real); subst equiv_a_a'_real; [solve [mauto]| |]; *)
-(*     intros * equiv_c_c'; unfold per_elem, Per_univ_def.per_elem in equiv_c_c'; destruct (rel_B_B' _ _ equiv_c_c'). *)
-(*   - econstructor; only 1-2: solve [mauto]. *)
-(*     intros b b' eval_B eval_B'. *)
-(*     econstructor; apply H. *)
-(*     Unshelve. *)
-(*     3-5: eassumption. *)
-(*   - econstructor; only 1-2: solve [mauto]. *)
-(*     intros b b' eval_B eval_B'. *)
-(*     eapply H0; solve [mauto]. *)
-(* Qed. *)
+From Equations Require Import Equations.
 
 Lemma per_univ_sym : forall m m' i,
-    {{ Dom m ≈ m' ∈ per_univ i }} ->
-    {{ Dom m' ≈ m ∈ per_univ i }}
-with per_elem_sym : forall m m' i R R'
+    {{ Dom m ≈ m' ∈ per_univ i }} -> {{ Dom m' ≈ m ∈ per_univ i }}
+with per_elem_sym : forall m m' i R R' a a'
   (equiv_m_m' : {{ DF m ≈ m' ∈ per_univ_elem i ↘ R }})
   (equiv_m'_m : {{ DF m' ≈ m ∈ per_univ_elem i ↘ R' }}),
-    {{ Dom m ≈ m' ∈ R }} ->
-    {{ Dom m' ≈ m ∈ R' }}.
+    {{ Dom a ≈ a' ∈ R }} <-> {{ Dom a' ≈ a ∈ R' }}.
 Proof with mauto.
-  - intros.
-    destruct H as [per_elem Hper_univ].
-    unfold in_dom_fun_rel in *.
-    dependent induction Hper_univ; try solve [subst; eexists; econstructor; mauto].
-    + fold per_univ_elem in equiv_a_a'.
-    (*   eexists; econstructor... *)
-    (* +  *)
-    (* unfold per_univ, Per_univ_def.per_univ, in_dom_rel in *. *)
-    (* destruct H as [equiv_a_a' Hcheck]. *)
-    (* dependent induction Hcheck; subst. *)
-    (* + eexists. *)
-    (*   eapply Per_univ_def.per_univ_check_univ. *)
-    (*   Unshelve. all: auto. *)
-    (* + eexists. *)
-    (*   econstructor. *)
-    (* + destruct IHHcheck. *)
-    (*   assert (Per_univ_def.per_univ_template i d{{{ Π a' p' B'}}} d{{{ Π a p B}}}). *)
-    (*   { eapply (@Per_univ_def.per_univ_template_pi i _ _ _ _ _ _ (per_univ i) (fun _ _ => per_elem) (ex_intro _ x H1)). *)
-    (*     intros. *)
-    (*     unfold in_dom_rel, per_elem, Per_univ_def.per_elem in *. *)
-    (*   } *)
+  all: intros *; try split.
+  1: intro Hper_univ.
+  2-3: intro Hper_elem.
+  - destruct Hper_univ as [per_elem equiv_m_m'].
+    autorewrite with per_univ_elem in equiv_m_m'.
+    dependent induction equiv_m_m'; subst; only 1-2,4: solve [eexists; econstructor; mauto].
+    (* Pi case *)
+    destruct IHequiv_m_m' as [in_rel' IHequiv_a_a'].
+    rewrite <- per_univ_elem_equation_1 in H, equiv_a_a'.
+    (* (* One attempt *) *)
+    (* unshelve epose (out_rel' := _ : forall c' c : domain, {{ Dom c' ≈ c ∈ in_rel' }} -> relation domain). *)
+    (* { *)
+    (*   intros * equiv_c'_c. *)
+    (*   assert (equiv_c_c' : {{ Dom c ≈ c' ∈ in_rel }}) by (erewrite per_elem_sym; eassumption). *)
+    (*   assert (rel_mod_eval (per_univ_elem i) B d{{{ p ↦ c }}} B' d{{{ p' ↦ c' }}} (out_rel c c' equiv_c_c')) by mauto. *)
+    (*   (* Failure point *) *)
+    (*   destruct_last. *)
+    (* } *)
+
+    (* (* The other *) *)
+    (* assert (exists (out_rel' : forall c' c : domain, {{ Dom c' ≈ c ∈ in_rel' }} -> relation domain), *)
+    (*          forall (c' c : domain) (equiv_c'_c : {{ Dom c' ≈ c ∈ in_rel' }}), *)
+    (*            rel_mod_eval (per_univ_elem i) B' d{{{ p' ↦ c' }}} B d{{{ p ↦ c }}} (out_rel' c' c equiv_c'_c)). *)
+    (* { *)
+    (*   (* This "eexists" is problematic *) *)
     (*   eexists. *)
-    (*   econstructor. *)
-    (*   * eassumption. *)
-    (*   * intros. *)
+    (*   intros. *)
+    (*   assert (equiv_c_c' : {{ Dom c ≈ c' ∈ in_rel }}) by (erewrite per_elem_sym; eassumption). *)
+    (*   assert (rel_mod_eval (per_univ_elem i) B d{{{ p ↦ c }}} B' d{{{ p' ↦ c' }}} (out_rel c c' equiv_c_c')) by mauto. *)
+    (*   destruct_last. *)
+    (*   econstructor; try eassumption. *)
+    (* } *)
       
